(см. [[Классы элементарных функций]] и [[Понятие производной]])

(1) $$y = \sin x$$

$$
(\sin x)' = \lim_{\Delta x→0} \frac{\sin(x+\Delta x) - \sin x}{\Delta x} = \lim_{\Delta x→0} \frac{2\sin(\frac{x + \Delta x - x}{2})\cos(\frac{x + \Delta x + x}{2})}{\Delta x} = 
$$

$$
= \lim_{\Delta x→0} \frac{2\sin(\frac{\Delta x}2)\cos(\frac{2x + \Delta x}{2})}{\Delta x} = \lim_{\Delta x→0} \frac{\sin(\frac{\Delta x}{2}) \cos(\frac{2x + \Delta x}{2})}{\frac{\Delta x}{2}} = 
$$

$$
= \lim_{\Delta x→0} \cos(\frac{2x + \Delta x}{2}) = \cos(\frac{2x}2) = \cos x
$$

(2) $$y = \cos x$$

$$
(\cos x)' = \lim_{\Delta x→0} \frac{\cos(x + \Delta x) - \cos x}{\Delta x} = \lim_{\Delta x→0} \frac{2\sin(\frac{x + \Delta x + x}{2})\sin(\frac{x - x - \Delta x}{2})}{\Delta x} =
$$

$$
= \lim_{\Delta x→0} \frac{2\sin(\frac{2x + \Delta x}{2})\sin(\frac{-\Delta x}{2})}{\Delta x} = \lim_{\Delta x→0} \frac{-\sin(\frac{2x + \Delta x}{x})\sin(\frac{\Delta x}{2})}{\frac{\Delta x}{2}} =
$$

$$
\lim_{\Delta x→0} -\sin(\frac{2x + \Delta x}{2}) = -\sin(\frac{2x}2) = -\sin x
$$

(3) $$y = \operatorname{tg} x$$

$$
(\operatorname{tg} x)' = (\frac{\sin x}{\cos x})' = \frac{(\sin x)'(\cos x) - (\sin x)(\cos x)'}{\cos^2 x} = \frac{\cos^2 x + \sin^2 x}{\cos^2 x} = \frac{1}{cos^2 x}
$$

(4) $$y = \operatorname{ctg} x$$

$$
(\operatorname{ctg} x)' = (\frac{\cos x}{\sin x})' = \frac{(\cos x)'(\sin x) - (\cos x)(\sin x)'}{\sin^2 x} = \frac{- \sin^2 x - \cos^2 x}{\sin^2 x} = -\frac{1}{sin^2 x}
$$

(5) $$y = \arcsin x$$

Используем формулу производной обратной функции $x = \sin y$:

$$
y'_x = \frac{1}{x'_y} = \frac{1}{\cos y} = \frac{1}{\sqrt{1 - sin^2 y}} = \frac{1}{\sqrt{1 - x^2}}
$$

(6) $$y = \arccos x$$

Используем формулу производной обратной функции $x = \cos y$:

$$
y'_x = \frac{1}{x'_y} = \frac{1}{-\sin y} = \frac{1}{-\sqrt{1 - cos^2 y}} = -\frac{1}{\sqrt{1 - x^2}}
$$

(7) $$y = \operatorname{arctg} x$$

Используем формулу производной обратной функции $x = \operatorname{tg} y$:

$$
y'_x = \frac{1}{x'_y} = \frac{1}{\frac{1}{cos^2 y}} = \frac{1}{\frac{\sin^2 y + \cos^2 y}{cos^2 y}} = \frac{1}{1 + \operatorname{tg}^2 y} = \frac{1}{1 + x^2}
$$

(8) $$y = \operatorname{arcctg} x$$

Используем формулу производной обратной функции $x = \operatorname{ctg} y$:

$$
y'_x = \frac{1}{x'_y} = \frac{1}{-\frac{1}{sin^2 y}} = \frac{1}{-\frac{\sin^2 y + \cos^2 y}{sin^2 y}} = -\frac{1}{1 + \operatorname{ctg}^2 y} = -\frac{1}{1 + x^2}
$$

(9) $$y = \log_a x$$

$$
(\log_a x)' = \lim_{\Delta x→0} \frac{\log_a (x + \Delta x) - \log_a x}{\Delta x} = \lim_{\Delta x→0} (\frac{1}{\Delta x}\log_a(\frac{x + \Delta x}{x})) = 
$$

$$
= \lim_{\Delta x→0}(\log_a(\frac{x + \Delta x}{x})^{\frac{1}{\Delta x}}) = \lim_{\Delta x→0}(\log_a(1 + \frac{\Delta x}{x})^{\frac{x}{\Delta x}\frac{1}{x}})) = \lim_{\Delta x→0}(\log_a(1 + \frac{1}{\frac{x}{\Delta x}})^{\frac{x}{\Delta x}\frac{1}{x}})) = 
$$

$$
= \lim_{\Delta x→0} (\log_a e)^{\frac{1}{x}} = \frac{1}{x}\log_a e = \frac{1}{x} \frac{1}{\ln a} = \frac{1}{x\ln a}
$$

(9.1) $$y = \ln x$$

$$
(\ln x)' = (\log_e x)' = \frac{1}{x \ln e} = \frac{1}{x}
$$

(10) $$y = a^x$$

Используем формулу производной обратной функции $x = \log_a y$:

$$
y'_x = \frac{1}{x'_y} = \frac{1}{\frac{1}{y \ln a}} = y \ln a = a^x \ln a
$$

(10.1) $$y = e^x$$

$$
(e^x)' = e^x \ln e = e^x
$$

(11) $$y = x^p$$

$$
(x^p)' = (e^{\ln x^p})' = (e^{p \ln x})' = e^{p \ln x} · (p \ln x)' = (e^{\ln x})^p · p · \frac{1}{x} =  p · \frac{x^p}{x} = px^{p-1}
$$

